Pushing insertion implementation
Also adding lemma names

model/BTrees.v
@@ -357,11 +357,55 @@ Fixpoint insert_up (s : splitpair) (cn : list nat) (cf : list treelist) : cursor
   | (_,_) => ([],[])
   end.
 
+Fixpoint insert_val (x : key) (v : V) (n : nat) (f : treelist) : nat * treelist :=
+  match f with
+  | tl_cons (val k v') f =>
+    (match n with
+     | O => if eq_key k x then (O, tl_cons (val k v) f)
+            else (S O, tl_cons (val x v) (tl_cons (val k v') f))
+     | S n => match insert_val x v n f with (n, f) => (S n, tl_cons (val k v') f) end
+     end)
+  | tl_nil => (S O, tl_cons (val x v) tl_nil)
+  | _ => (S O, tl_cons (val x v) tl_nil) (* should never happen *)
+  end.
+
 (* Needs to point the cursor to the right place (if it's straddling a leaf divide) *)
 (* Then, insert (x,v) in (either replacing next or inserting before it) *)
 (* Needs to bump the first n up to be past what was just inserted *)
 (* Finally, turns that treelist into a splitpair and calls insert_up. *)
-Fixpoint insert (x : key) (v : V) (c : cursor) : cursor := ([],[]).
+Fixpoint insert (x : key) (v : V) (c : cursor) : cursor :=
+  match c with
+  | (n::cn,f::cf) =>
+    (match next_node cn cf with
+      | Some ((n'::cn',f'::cf'),k) =>
+        if lt_key x k then (match insert_val x v n f with (n,f) =>
+          (match decide_split f with 
+           | One f => (match insert_up (One f) cn cf with (cn,cf) => (n::cn,f::cf) end)
+           | Two f1 k f2 =>
+             (match insert_up (Two f1 k f2) cn cf with (cn,cf) =>
+              if (Nat.leb (treelist_length f1) n) then ((n-(treelist_length f1))::cn, f2::cf)
+              else (n::cn,f1::cf) end)
+           end) end)
+        else (match insert_val x v n' f' with (n',f') =>
+          (match decide_split f' with
+           | One f' => (match insert_up (One f') cn' cf' with (cn',cf') => (n'::cn',f'::cf') end)
+           | Two f1 k f2 =>
+             (match insert_up (Two f1 k f2) cn' cf' with (cn',cf') =>
+              if (Nat.leb (treelist_length f1) n) then ((n-(treelist_length f1))::cn, f2::cf)
+              else (n::cn,f1::cf) end)
+           end) end)
+      | None => (match insert_val x v n f with (n,f) =>
+        (match decide_split f with 
+         | One f => (match insert_up (One f) cn cf with (cn,cf) => (n::cn,f::cf) end)
+         | Two f1 k f2 =>
+           (match insert_up (Two f1 k f2) cn cf with (cn,cf) =>
+            if (Nat.leb (treelist_length f1) n) then ((n-(treelist_length f1))::cn, f2::cf)
+            else (n::cn,f1::cf) end)
+         end) end)
+      | _ => ([],[]) (* shouldn't be possible *)
+      end)
+  | _=> ([S O], [tl_cons (val x v) tl_nil]) (* tree must be empty *)
+  end.
 
 (** CURSOR_ELEMENTS *)
 
@@ -688,6 +732,7 @@ Definition cursor_correct (c : cursor) : Prop :=
   * Proofs about this abstraction and the implementation
   *)
 
+(* Lemma 1 in the doc *)
 (* Proof that splitting into sides is equivalent -- now I can prove about the sides separately! *)
 Theorem cursor_elements'_sides_equiv : forall cn cf l r,
   cursor_elements' cn cf l r = (cursor_left cn cf l, cursor_right cn cf r).
@@ -703,6 +748,7 @@ Definition right_el_P (t : tree) : Prop := forall k f b,
   t = node k f \/ t = final f ->
   exists l', right_el f b = b++l'.
 
+(* Lemma 2 *)
 Theorem right_el_interior : forall f b,
   exists l', right_el f b = b++l'.
 Proof.
@@ -730,6 +776,7 @@ Definition left_el_P (t : tree) : Prop := forall k f b,
   t = node k f \/ t = final f ->
   exists l', left_el f b = b++l'.
 
+(* Lemma 2 *)
 Theorem left_el_interior : forall f b,
   exists l', left_el f b = b++l'.
 Proof.
@@ -753,6 +800,7 @@ Proof.
       exists (x++[(k,v)]). rewrite <- app_assoc. reflexivity.
 Qed.
 
+(* Lemma 2 *)
 Theorem left_rec_interior : forall cn cf l,
   exists l', cursor_left cn cf l = (l++l').
 Proof.
@@ -766,6 +814,7 @@ Proof.
     inversion H0. rewrite H1. exists (x0++x). rewrite app_assoc. reflexivity.
 Qed.
 
+(* Lemma 2 *)
 Theorem right_rec_interior : forall cn cf r,
   exists r', cursor_right cn cf r = (r++r').
 Proof.
@@ -803,7 +852,7 @@ Proof.
 Qed.
 *)
 
-
+(* Lemma 3 *)
 (* If you split a list, the result of the elements of the first with the elements of the second is the same *)
 Theorem cursor_right_elements1 : forall cn1 cf1 cn2 cf2 b,
   length cn1 = length cf1 -> length cn2 = length cf2 ->
@@ -831,372 +880,41 @@ Proof.
     apply IHcn1. apply H2. apply H0.
 Qed.
 
-(* Having 0 & f puts nothing on the left, elements of f on the right *)
-Theorem cursor_right_elements2 : forall f cn cf b,
-  cursor_right (O::cn) (f::cf) b = cursor_right cn cf (right_el f b).
-Proof. Admitted. (* This isn't quite the right statement *)
+(* List in increasing order *)
+Inductive sorted_less : list (key * V) -> Prop :=
+| sl_nil : sorted_less []
+| sl_one : forall k v, sorted_less [(k,v)]
+| sl_next : forall k1 v1 k2 v2 l,
+  lt_key k1 k2 = true -> sorted_less ((k2,v2)::l) -> sorted_less ((k1,v1)::(k2,v2)::l).
 
-Theorem cursor_left_elements2 : forall f cn cf b,
-  cursor_left (O::cn) (f::cf) b = cursor_left cn cf b.
-Proof. destruct f; reflexivity. Qed.
+(* List in decreasing order *)
+Inductive sorted_more : list (key * V) -> Prop :=
+| sm_nil : sorted_more []
+| sm_one : forall k v, sorted_more [(k,v)]
+| sm_next : forall k1 v1 k2 v2 l,
+  lt_key k2 k1 = true -> sorted_more ((k2,v2)::l) -> sorted_more ((k1,v1)::(k2,v2)::l).
 
-(* Having n & f where n is past the end of the list, elements of f on the left & nothing on the right *)
-Theorem cursor_right_elements3 : forall cn cf n f b,
-  n >= treelist_length f ->
-  cursor_right (n::cn) (f::cf) b = cursor_right cn cf b.
-Proof.
-  intros. apply point_treelist_length in H.
-  simpl. inversion H. rewrite H0. reflexivity.
-Qed.
+(* Theorem 4 *)
+Theorem cursor_right_el_sorted : forall cn cf,
+  cursor_correct (cn,cf) -> sorted_less (cursor_right cn cf []).
+Proof. Admitted.
 
-(* For cursor_elements' [n] [f], it's equal to *)
+(* Theorem 4 *)
+Theorem cursor_left_el_sorted : forall cn cf,
+  cursor_correct (cn,cf) -> sorted_more (cursor_left cn cf []).
+Proof. Admitted.
 
-Theorem next_correct_struct : forall cn cf c,
-  cursor_correct_struct (cn,cf) -> next_node cn cf = Some c -> cursor_correct_struct c.
-Proof.
-  induction cn,cf.
-  - intros; simpl. simpl in H0. inversion H0.
-  - intros; simpl. inversion H.
-  - intros; simpl. inversion H.
-  - intros. inversion H.
-    + subst. simpl in H0. destruct (point a t) eqn:e. destruct p.
-      destruct o. destruct t2; destruct t0; try (inversion H0).
-      destruct t0; inversion H0; apply cc_first.
-      destruct t0; inversion H0; apply cc_first.
-      apply cc_first.
-      destruct t0; inversion H0; apply cc_first.
-      destruct t0. inversion H0. destruct t0; inversion H0; apply cc_first.
-    + subst. remember (n::ci) as cn'. remember (f::ct) as cf'.
-      simpl in H0. destruct (point a t) eqn:e. destruct p.
-      destruct o; destruct t0.
-      * destruct t2. destruct (next_node cn' cf') eqn:e2. destruct c0.
-        destruct l. inversion H0. destruct l0. inversion H0.
-        destruct (point n0 t2) eqn:e3. destruct p. destruct o. destruct t5.
-        { inversion H0. apply cc_node with k1. apply IHcn with cf'. inversion H.
-          apply cc_nil. apply H5. apply H5. apply e2. apply point_lin_search with t4 t3. apply e3. }
-        { inversion H0. apply cc_final. apply IHcn with cf'. inversion H.
-          apply cc_nil. apply H5. apply H5. apply e2. apply point_lin_search with t4 t3. apply e3. }
-        { inversion H0. }
-        { inversion H0. }
-        { inversion H0. }
-        destruct (next_node cn' cf') eqn:e2. destruct c0.
-        destruct l. inversion H0. destruct l0. inversion H0.
-        destruct (point n0 t2) eqn:e3. destruct p. destruct o. destruct t5.
-        { inversion H0. apply cc_node with k0. apply IHcn with cf'. inversion H.
-          apply cc_nil. apply H5. apply H5. apply e2. apply point_lin_search with t4 t3. apply e3. }
-        { inversion H0. apply cc_final. apply IHcn with cf'. inversion H.
-          apply cc_nil. apply H5. apply H5. apply e2. apply point_lin_search with t4 t3. apply e3. }
-        { inversion H0. }
-        { inversion H0. }
-        { inversion H0. }
-        inversion H0. apply H.
-      * destruct t2; destruct t0.
-        { inversion H0. inversion H. apply cc_first. apply cc_node with k2.
-          apply H5. apply H9. apply cc_final. apply H5. apply H9. }
-        { inversion H0. inversion H. apply cc_first. apply cc_node with k1.
-          apply H5. apply H9. apply cc_final. apply H5. apply H9. }
-        destruct (next_node cn' cf') eqn:e2. destruct c0.
-        destruct l. inversion H0. destruct l0. inversion H0.
-        destruct (point n0 t0) eqn:e3. destruct p. destruct o. destruct t6.
-        { inversion H0. apply cc_node with k2. apply IHcn with cf'. inversion H.
-          apply cc_nil. apply H5. apply H5. apply e2. apply point_lin_search with t5 t4. apply e3. }
-        { inversion H0. apply cc_final. apply IHcn with cf'. inversion H.
-          apply cc_nil. apply H5. apply H5. apply e2. apply point_lin_search with t5 t4. apply e3. }
-        { inversion H0. }
-        { inversion H0. }
-        { inversion H0. }
-        { inversion H0. inversion H. apply cc_first. apply cc_node with k1.
-          apply H5. apply H9. apply cc_final. apply H5. apply H9. }
-        { inversion H0. inversion H. apply cc_first. apply cc_node with k0.
-          apply H5. apply H9. apply cc_final. apply H5. apply H9. }
-        destruct (next_node cn' cf') eqn:e2. destruct c0.
-        destruct l. inversion H0. destruct l0. inversion H0.
-        destruct (point n0 t0) eqn:e3. destruct p. destruct o. destruct t6.
-        { inversion H0. apply cc_node with k1. apply IHcn with cf'. inversion H.
-          apply cc_nil. apply H5. apply H5. apply e2. apply point_lin_search with t5 t4. apply e3. }
-        { inversion H0. apply cc_final. apply IHcn with cf'. inversion H.
-          apply cc_nil. apply H5. apply H5. apply e2. apply point_lin_search with t5 t4. apply e3. }
-        { inversion H0. }
-        { inversion H0. }
-        { inversion H0. }
-        { inversion H0. inversion H. apply cc_first. apply cc_node with k2.
-          apply H5. apply H9. apply cc_final. apply H5. apply H9. }
-        { inversion H0. inversion H. apply cc_first. apply cc_node with k1.
-          apply H5. apply H9. apply cc_final. apply H5. apply H9. }
-        { inversion H0. apply H. }
-      * destruct (next_node cn' cf') eqn:e2. destruct c0.
-        destruct l. inversion H0. destruct l0. inversion H0.
-        destruct (point n0 t0) eqn:e3. destruct p. destruct o. destruct t4.
-        { inversion H0. apply cc_node with k0. apply IHcn with cf'. inversion H.
-          apply cc_nil. apply H5. apply H5. apply e2. apply point_lin_search with t3 t2. apply e3. }
-        { inversion H0. apply cc_final. apply IHcn with cf'. inversion H.
-          apply cc_nil. apply H5. apply H5. apply e2. apply point_lin_search with t3 t2. apply e3. }
-        { inversion H0. }
-        { inversion H0. }
-        { inversion H0. }
-      * apply point_none in e. inversion e.
-    + subst. remember (n::ci) as cn'. remember (f::ct) as cf'.
-      simpl in H0. destruct (point a t) eqn:e. destruct p.
-      destruct o; destruct t0.
-      * destruct t2. destruct (next_node cn' cf') eqn:e2. destruct c0.
-        destruct l. inversion H0. destruct l0. inversion H0.
-        destruct (point n0 t2) eqn:e3. destruct p. destruct o. destruct t5.
-        { inversion H0. apply cc_node with k0. apply IHcn with cf'. inversion H.
-          apply cc_nil. apply H5. apply H5. apply e2. apply point_lin_search with t4 t3. apply e3. }
-        { inversion H0. apply cc_final. apply IHcn with cf'. inversion H.
-          apply cc_nil. apply H5. apply H5. apply e2. apply point_lin_search with t4 t3. apply e3. }
-        { inversion H0. }
-        { inversion H0. }
-        { inversion H0. }
-        destruct (next_node cn' cf') eqn:e2. destruct c0.
-        destruct l. inversion H0. destruct l0. inversion H0.
-        destruct (point n0 t2) eqn:e3. destruct p. destruct o. destruct t5.
-        { inversion H0. apply cc_node with k. apply IHcn with cf'. inversion H.
-          apply cc_nil. apply H5. apply H5. apply e2. apply point_lin_search with t4 t3. apply e3. }
-        { inversion H0. apply cc_final. apply IHcn with cf'. inversion H.
-          apply cc_nil. apply H5. apply H5. apply e2. apply point_lin_search with t4 t3. apply e3. }
-        { inversion H0. }
-        { inversion H0. }
-        { inversion H0. }
-        inversion H0. apply H.
-      * destruct t2; destruct t0.
-        { inversion H0. inversion H. apply cc_first. apply cc_node with k1.
-          apply H5. apply H9. apply cc_final. apply H5. apply H9. }
-        { inversion H0. inversion H. apply cc_first. apply cc_node with k0.
-          apply H5. apply H9. apply cc_final. apply H5. apply H9. }
-        destruct (next_node cn' cf') eqn:e2. destruct c0.
-        destruct l. inversion H0. destruct l0. inversion H0.
-        destruct (point n0 t0) eqn:e3. destruct p. destruct o. destruct t6.
-        { inversion H0. apply cc_node with k1. apply IHcn with cf'. inversion H.
-          apply cc_nil. apply H5. apply H5. apply e2. apply point_lin_search with t5 t4. apply e3. }
-        { inversion H0. apply cc_final. apply IHcn with cf'. inversion H.
-          apply cc_nil. apply H5. apply H5. apply e2. apply point_lin_search with t5 t4. apply e3. }
-        { inversion H0. }
-        { inversion H0. }
-        { inversion H0. }
-        { inversion H0. inversion H. apply cc_first. apply cc_node with k0.
-          apply H5. apply H9. apply cc_final. apply H5. apply H9. }
-        { inversion H0. inversion H. apply cc_first. apply cc_node with k.
-          apply H5. apply H9. apply cc_final. apply H5. apply H9. }
-        destruct (next_node cn' cf') eqn:e2. destruct c0.
-        destruct l. inversion H0. destruct l0. inversion H0.
-        destruct (point n0 t0) eqn:e3. destruct p. destruct o. destruct t6.
-        { inversion H0. apply cc_node with k0. apply IHcn with cf'. inversion H.
-          apply cc_nil. apply H5. apply H5. apply e2. apply point_lin_search with t5 t4. apply e3. }
-        { inversion H0. apply cc_final. apply IHcn with cf'. inversion H.
-          apply cc_nil. apply H5. apply H5. apply e2. apply point_lin_search with t5 t4. apply e3. }
-        { inversion H0. }
-        { inversion H0. }
-        { inversion H0. }
-        { inversion H0. inversion H. apply cc_first. apply cc_node with k1.
-          apply H5. apply H9. apply cc_final. apply H5. apply H9. }
-        { inversion H0. inversion H. apply cc_first. apply cc_node with k0.
-          apply H5. apply H9. apply cc_final. apply H5. apply H9. }
-        { inversion H0. apply H. }
-      * destruct (next_node cn' cf') eqn:e2. destruct c0.
-        destruct l. inversion H0. destruct l0. inversion H0.
-        destruct (point n0 t0) eqn:e3. destruct p. destruct o. destruct t4.
-        { inversion H0. apply cc_node with k. apply IHcn with cf'. inversion H.
-          apply cc_nil. apply H5. apply H5. apply e2. apply point_lin_search with t3 t2. apply e3. }
-        { inversion H0. apply cc_final. apply IHcn with cf'. inversion H.
-          apply cc_nil. apply H5. apply H5. apply e2. apply point_lin_search with t3 t2. apply e3. }
-        { inversion H0. }
-        { inversion H0. }
-        { inversion H0. }
-      * apply point_none in e. inversion e.
-Qed.
+(* Theorem 5 *)
+Theorem cursor_right_el_complete : True.
+Proof. Admitted.
 
-Lemma balance_carries_one : forall n f k f',
-  balanced f ->
-  (lin_search n f = Some (node k f') \/ lin_search n f = Some (final f')) ->
-  balanced f'.
-Proof.
-  induction n; intros; destruct f.
-  - inversion H0; inversion H1.
-  - inversion H0; inversion H1; rewrite H3 in H; inversion H; inversion H2; subst.
-    unfold balanced. exists n. apply H7.
-    unfold balanced. exists n. apply H6.
-  - inversion H0; inversion H1.
-  - simpl in H0. apply IHn with f k.
-    + inversion H. inversion H1; subst.
-      exists 1. apply H4.
-      exists (S n0). apply H6.
-      exists 1. apply bf_nil.
-    + apply H0.
-Qed.
+(* Theorem 5 *)
+Theorem cursor_left_el_complete : True.
+Proof. Admitted.
 
-Lemma balance_carries : forall cn cf n f,
-  cursor_correct_struct (n::cn,f::cf) ->
-  rec_prop balanced (cn,cf) ->
-  cn <> [] ->
-  rec_prop balanced (n::cn,f::cf).
-Proof.
-  intros. inversion H0. destruct H1. auto.
-  subst. apply rp_next. 2:apply H0.
-  inversion H4. inversion H.
-  - subst. apply balance_carries_one with n0 f0 k. apply H4. left. apply H12.
-  - subst. apply balance_carries_one with n0 f0 Z0. apply H4. right. apply H12.
-Qed.
+(** Theorems about next_node and prev_node *)
 
-Theorem next_node_balanced : forall cn cf c,
-  cursor_correct_struct (cn,cf) -> rec_prop balanced (cn,cf) ->
-  next_node cn cf = Some c -> rec_prop balanced c.
-Proof.
-  induction cn,cf; intros.
-  - inversion H1.
-  - inversion H1.
-  - inversion H1.
-  - inversion H0. subst.
-    assert (cursor_correct_struct (cn,cf)).
-    { inversion H; subst. apply cc_nil. apply H5. apply H5. }
-    assert (IHpart: forall c, next_node cn cf = Some c -> rec_prop balanced c).
-    { intros. apply IHcn with cf. apply H2. apply H7. apply H3. }
-    assert (cursor_correct_struct c).
-    { apply next_correct_struct with (a::cn) (t::cf). apply H. apply H1. }
-    inversion H1. destruct (point a t) eqn:e1. destruct p.
-    destruct o; try (destruct t2); destruct t0.
-    + destruct (next_node cn cf) eqn:e2. destruct c0. destruct l. 2:destruct l0.
-      inversion H6. inversion H6. destruct (point n t0). destruct p.
-      2:inversion H6. destruct o. 2:inversion H6. destruct t5. 3:inversion H6.
-      * inversion H6. apply balance_carries.
-        rewrite H8. apply H3.
-        apply IHpart. reflexivity.
-        intros Hcontra. inversion Hcontra.
-      * inversion H6. apply balance_carries.
-        rewrite H8. apply H3.
-        apply IHpart. reflexivity.
-        intros Hcontra. inversion Hcontra.
-    + destruct t0.
-      { inversion H6. apply rp_next. apply H4. apply H7. }
-      { inversion H6. apply rp_next. apply H4. apply H7. }
-      destruct (next_node cn cf) eqn:e2. destruct c0. destruct l. 2:destruct l0.
-      inversion H6. inversion H6. 2:inversion H6.
-      destruct (point n t0) eqn:e3. destruct p. destruct o. destruct t6.
-      { inversion H6. apply balance_carries.
-        rewrite H8. apply H3.
-        apply IHpart. reflexivity.
-        intros Hcontra. inversion Hcontra. }
-      { inversion H6. apply balance_carries.
-        rewrite H8. apply H3.
-        apply IHpart. reflexivity.
-        intros Hcontra. inversion Hcontra. }
-      inversion H6. inversion H6.
-    + destruct (next_node cn cf) eqn:e2. destruct c0. destruct l. 2:destruct l0.
-      inversion H6. inversion H6. destruct (point n t0). destruct p.
-      2:inversion H6. destruct o. 2:inversion H6. destruct t5. 3:inversion H6.
-      * inversion H6. apply balance_carries.
-        rewrite H8. apply H3.
-        apply IHpart. reflexivity.
-        intros Hcontra. inversion Hcontra.
-      * inversion H6. apply balance_carries.
-        rewrite H8. apply H3.
-        apply IHpart. reflexivity.
-        intros Hcontra. inversion Hcontra.
-    + destruct t0.
-      { inversion H6. apply rp_next. apply H4. apply H7. }
-      { inversion H6. apply rp_next. apply H4. apply H7. }
-      destruct (next_node cn cf) eqn:e2. destruct c0. destruct l. 2:destruct l0.
-      inversion H6. inversion H6. 2:inversion H6.
-      destruct (point n t0) eqn:e3. destruct p. destruct o. destruct t6.
-      { inversion H6. apply balance_carries.
-        rewrite H8. apply H3.
-        apply IHpart. reflexivity.
-        intros Hcontra. inversion Hcontra. }
-      { inversion H6. apply balance_carries.
-        rewrite H8. apply H3.
-        apply IHpart. reflexivity.
-        intros Hcontra. inversion Hcontra. }
-      inversion H6. inversion H6.
-    + inversion H6. apply H0.
-    + destruct t0.
-      * inversion H6. apply rp_next. apply H4. apply H7.
-      * inversion H6. apply rp_next. apply H4. apply H7.
-      * inversion H6. apply H0.
-    + destruct (next_node cn cf) eqn:e2. destruct c0. destruct l. 2:destruct l0.
-      inversion H6. inversion H6. destruct (point n t0). destruct p.
-      2:inversion H6. destruct o. 2:inversion H6. destruct t4. 3:inversion H6.
-      * inversion H6. apply balance_carries.
-        rewrite H8. apply H3.
-        apply IHpart. reflexivity.
-        intros Hcontra. inversion Hcontra.
-      * inversion H6. apply balance_carries.
-        rewrite H8. apply H3.
-        apply IHpart. reflexivity.
-        intros Hcontra. inversion Hcontra.
-    + destruct t0.
-      { inversion H6. apply rp_next. apply H4. apply H7. }
-      { inversion H6. apply rp_next. apply H4. apply H7. }
-      destruct (next_node cn cf) eqn:e2. destruct c0. destruct l. 2:destruct l0.
-      inversion H6. inversion H6. 2:inversion H6.
-      destruct (point n t0) eqn:e3. destruct p. destruct o. destruct t5.
-      { inversion H6. apply balance_carries.
-        rewrite H8. apply H3.
-        apply IHpart. reflexivity.
-        intros Hcontra. inversion Hcontra. }
-      { inversion H6. apply balance_carries.
-        rewrite H8. apply H3.
-        apply IHpart. reflexivity.
-        intros Hcontra. inversion Hcontra. }
-      inversion H6. inversion H6.
-Qed.
-
-Lemma next_node_none : forall cn cf cn' cf',
-  next_node cn cf = Some (cn',cf') ->
-  cn' <> [] /\ cf' <> [].
-Proof.
-  induction cn,cf; intros.
-  - simpl in H. inversion H.
-  - simpl in H. inversion H.
-  - simpl in H. inversion H.
-  - simpl in H. destruct (point a t) eqn:e. destruct p.
-    destruct t0; destruct o. destruct t0.
-    * destruct (next_node cn cf) eqn:e2. destruct c; destruct l. 2:destruct l0.
-      inversion H. inversion H.
-      destruct (point n t2) eqn:e3. destruct p.
-      destruct o; try (destruct t5); inversion H; split; intros Hcontra; inversion Hcontra.
-      inversion H.
-    * destruct (next_node cn cf) eqn:e2. destruct c; destruct l. 2:destruct l0.
-      inversion H. inversion H.
-      destruct (point n t2) eqn:e3. destruct p.
-      destruct o; try (destruct t5); inversion H; split; intros Hcontra; inversion Hcontra.
-      inversion H.
-    * inversion H. split; intros Hcontra; inversion Hcontra.
-    * destruct (next_node cn cf) eqn:e2. destruct c; destruct l. 2:destruct l0.
-      inversion H. inversion H.
-      destruct (point n t0) eqn:e3. destruct p.
-      destruct o; try (destruct t4); inversion H; split; intros Hcontra; inversion Hcontra.
-      inversion H.
-    * destruct t3; destruct t0.
-      inversion H. split; intros Hcontra; inversion Hcontra.
-      inversion H. split; intros Hcontra; inversion Hcontra.
-      destruct (next_node cn cf) eqn:e2. destruct c; destruct l. 2:destruct l0.
-      inversion H. inversion H.
-      destruct (point n t0) eqn:e3. destruct p. destruct o. destruct t6.
-      inversion H. split; intros Hcontra; inversion Hcontra.
-      inversion H. split; intros Hcontra; inversion Hcontra.
-      inversion H. inversion H. inversion H.
-      inversion H. split; intros Hcontra; inversion Hcontra.
-      inversion H. split; intros Hcontra; inversion Hcontra.
-      destruct (next_node cn cf) eqn:e2. destruct c; destruct l. 2:destruct l0.
-      inversion H. inversion H.
-      destruct (point n t0) eqn:e3. destruct p. destruct o. destruct t6.
-      inversion H. split; intros Hcontra; inversion Hcontra.
-      inversion H. split; intros Hcontra; inversion Hcontra.
-      inversion H. inversion H. inversion H.
-      inversion H. split; intros Hcontra; inversion Hcontra.
-      inversion H. split; intros Hcontra; inversion Hcontra.
-      inversion H. split; intros Hcontra; inversion Hcontra.
-    * destruct t0.
-      inversion H. split; intros Hcontra; inversion Hcontra.
-      inversion H. split; intros Hcontra; inversion Hcontra.
-      destruct (next_node cn cf) eqn:e2. destruct c; destruct l. 2:destruct l0.
-      inversion H. inversion H.
-      destruct (point n t0) eqn:e3. destruct p. destruct o. destruct t5.
-      inversion H. split; intros Hcontra; inversion Hcontra.
-      inversion H. split; intros Hcontra; inversion Hcontra.
-      inversion H. inversion H. inversion H.
-Qed.
-
+(* Helper for Invariants *)
 Lemma point_next : forall f n f1 f1' f2 f2' o t,
   point n f = (f1, o, f2) ->
   point (S n) f = (f1', Some t, f2') ->
@@ -1214,9 +932,10 @@ Proof.
       apply IHf with n t2 t3 o. apply e. apply e'.
 Qed.
 
-Theorem cursor_right_elements4 : forall cn cf cn' cf' n f k f' t l1 l2 b,
+(* Invariant 6 *)
+Theorem cursor_right_elements4 : forall cn cf cn' cf' n f k f' t l1 l2 b k',
   cursor_correct_struct (cn,cf) ->
-  next_node cn cf = Some (n::cn',f::cf') ->
+  next_node cn cf = Some (n::cn',f::cf',k') ->
   (* (cn,cf) <> (n::cn',f::cf') -> *)
   point n f = (l1,Some t,l2) ->
   t = node k f' \/ t = final f' ->
@@ -1227,7 +946,7 @@ Proof.
   - simpl in H0. inversion H0.
   - simpl in H0. inversion H0.
   - simpl in H0. destruct (point a t) eqn:e. destruct p. destruct o; try (destruct t3); destruct t1.
-    + destruct (next_node cn cf) eqn:e2. destruct c; destruct l. 2:destruct l0.
+    + destruct (next_node cn cf) eqn:e2. destruct p. destruct c; destruct l. 2:destruct l0.
       * inversion H0.
       * inversion H0.
       * destruct (point n0 t1) eqn:e3. destruct p.
@@ -1236,7 +955,7 @@ Proof.
           simpl. rewrite e. destruct f. inversion H1.
           rewrite e3. simpl.
           assert (cursor_right cn cf b0 = cursor_right (n0::l) (t1::l0) (right_el (tl_cons t6 f) b0)).
-          { apply IHcn with k1 (node k1 (tl_cons t6 f)) t5 t4.
+          { apply IHcn with k2 (node k2 (tl_cons t6 f)) t5 t4 k'.
             inversion H. subst. apply cc_nil. apply H4. apply H4.
             apply e2.
             apply e3.
@@ -1247,7 +966,7 @@ Proof.
           simpl. rewrite e. destruct f. inversion H1.
           rewrite e3. simpl.
           assert (cursor_right cn cf b0 = cursor_right (n0::l) (t1::l0) (right_el (tl_cons t6 f) b0)).
-          { apply IHcn with k (final (tl_cons t6 f)) t5 t4.
+          { apply IHcn with k (final (tl_cons t6 f)) t5 t4 k'.
             inversion H. subst. apply cc_nil. apply H4. apply H4.
             apply e2.
             apply e3.
@@ -1260,16 +979,16 @@ Proof.
     + destruct t1.
       * inversion H0. subst. remember (S a) as a'. simpl. rewrite e. rewrite H1.
         assert (tl_cons (node k1 t1) t4 = tl_cons t0 l2).
-        { apply point_next with f a t2 l1 (Some (node k0 t3)). apply e. subst. apply H1. }
+        { apply point_next with f a t2 l1 (Some (node k' t3)). apply e. subst. apply H1. }
         inversion H3. subst. inversion H2; inversion H4. subst.
         simpl. reflexivity.
       * inversion H0. subst. remember (S a) as a'. simpl. rewrite e. rewrite H1.
         assert (tl_cons (final t1) t4 = tl_cons t0 l2).
-        { apply point_next with f a t2 l1 (Some (node k0 t3)). apply e. subst. apply H1. }
+        { apply point_next with f a t2 l1 (Some (node k' t3)). apply e. subst. apply H1. }
         inversion H3. subst. inversion H2; inversion H4. subst.
         simpl. reflexivity.
       * admit. (* e: node and val in same treelist *)
-    + destruct (next_node cn cf) eqn:e2. destruct c; destruct l. 2:destruct l0.
+    + destruct (next_node cn cf) eqn:e2. destruct p. destruct c; destruct l. 2:destruct l0.
       inversion H0.
       inversion H0.
       destruct (point n0 t1) eqn:e3. destruct p. destruct o. destruct t6.
@@ -1277,7 +996,7 @@ Proof.
         simpl. rewrite e. destruct f. inversion H1.
         rewrite e3. simpl.
         assert (cursor_right cn cf b0 = cursor_right (n0::l) (t1::l0) (right_el (tl_cons t6 f) b0)).
-          { apply IHcn with k0 (node k0 (tl_cons t6 f)) t5 t4.
+          { apply IHcn with k1 (node k1 (tl_cons t6 f)) t5 t4 k'.
             inversion H. subst. apply cc_nil. apply H4. apply H4.
             apply e2.
             apply e3.
@@ -1288,7 +1007,7 @@ Proof.
         simpl. rewrite e. destruct f. inversion H1.
         rewrite e3. simpl.
         assert (cursor_right cn cf b0 = cursor_right (n0::l) (t1::l0) (right_el (tl_cons t6 f) b0)).
-          { apply IHcn with k (final (tl_cons t6 f)) t5 t4.
+          { apply IHcn with k (final (tl_cons t6 f)) t5 t4 k'.
             inversion H. subst. apply cc_nil. apply H4. apply H4.
             apply e2.
             apply e3.
@@ -1298,10 +1017,46 @@ Proof.
       { inversion H0. }
       { inversion H0. }
       { inversion H0. }
-     + destruct t1.
+    + destruct (next_node cn cf) eqn:e2. destruct p. destruct c; destruct l. 2:destruct l0.
+      inversion H0.
+      inversion H0.
+      destruct (point n0 t5) eqn:e3. destruct p. destruct o. destruct t8.
+      { inversion H0. subst. clear H0.
+        simpl. rewrite e. destruct f. inversion H1.
+        rewrite e3. simpl. admit. }
+      admit. admit. admit. admit.
+    + admit.
+    + admit.
+    + admit.
+    + admit. (*
+        assert (cursor_right cn cf b0 = cursor_right (n0::l) (t1::l0) (right_el (tl_cons t6 f) b0)).
+          { apply IHcn with k1 (node k1 (tl_cons t6 f)) t5 t4 k'.
+            inversion H. subst. apply cc_nil. apply H4. apply H4.
+            apply e2.
+            apply e3.
+            left. reflexivity. }
+          rewrite H0. simpl. rewrite e3. simpl in H1. inversion H1. subst.
+          destruct H2. rewrite H2. reflexivity. rewrite H2. reflexivity. }
+      { inversion H0. subst. clear H0.
+        simpl. rewrite e. destruct f. inversion H1.
+        rewrite e3. simpl.
+        assert (cursor_right cn cf b0 = cursor_right (n0::l) (t1::l0) (right_el (tl_cons t6 f) b0)).
+          { apply IHcn with k (final (tl_cons t6 f)) t5 t4 k'.
+            inversion H. subst. apply cc_nil. apply H4. apply H4.
+            apply e2.
+            apply e3.
+            right. reflexivity. }
+          rewrite H0. simpl. rewrite e3. simpl in H1. inversion H1. subst.
+          destruct H2. rewrite H2. reflexivity. rewrite H2. reflexivity. }
+      { inversion H0. }
+      { inversion H0. }
+      { inversion H0. }
+
+
+       destruct t1.
        * inversion H0. subst. remember (S a) as a'. simpl. rewrite e. rewrite H1.
         assert (tl_cons (node k0 t1) t4 = tl_cons t0 l2).
-        { apply point_next with f a t2 l1 (Some (final t3)). apply e. subst. apply H1. }
+        { apply point_next with t a t2 l1 (Some (final t3)). apply e. subst. apply H1. }
         inversion H3. subst. inversion H2; inversion H4. subst.
         simpl. reflexivity.
       * inversion H0. subst. remember (S a) as a'. simpl. rewrite e. rewrite H1.
@@ -1344,9 +1099,10 @@ Proof.
       { inversion H0. }
       { inversion H0. }
       { inversion H0. }
-    + apply point_none in e. inversion e.
+    + apply point_none in e. inversion e. *)
 Admitted.
 
+(* Helper for invariant *)
 Lemma left_el_app : forall f1 f2 b,
   left_el (tl_app f1 f2) b = left_el f1 (left_el f2 b).
 Proof.
@@ -1355,9 +1111,10 @@ Proof.
   - simpl. rewrite IHf1. reflexivity.
 Qed.
 
-Theorem cursor_left_elements4 : forall cn cf cn' cf' n f b f1 o f2,
+(* Invariant 7 *)
+Theorem cursor_left_elements4 : forall cn cf cn' cf' n f b f1 o f2 k,
   cursor_correct_struct (n::cn,f::cf) ->
-  next_node (n::cn) (f::cf) = Some (cn',cf') ->
+  next_node (n::cn) (f::cf) = Some (cn',cf',k) ->
   (cn',cf') <> (n::cn,f::cf) ->
   point n f = (f1,o,f2) -> exists k f',
   (o = Some (node k f') /\ cursor_left (n::cn) (f::cf) (left_el f' b) = cursor_left cn' cf' b) \/
@@ -1366,7 +1123,7 @@ Theorem cursor_left_elements4 : forall cn cf cn' cf' n f b f1 o f2,
 Proof.
   induction cn,cf; intros.
   - simpl in H0. rewrite H2 in H0. destruct o. destruct t.
-    + exists k,t. left. split. reflexivity. destruct f2. 2:destruct t0. (* Note that these +s are basically all copies of each other*)
+    + exists k0,t. left. split. reflexivity. destruct f2. 2:destruct t0. (* Note that these +s are basically all copies of each other*)
       * inversion H0.
       * inversion H0. remember (S n) as n'. simpl.
         destruct (point n f) eqn:e1. destruct p.
@@ -1383,9 +1140,17 @@ Proof.
           rewrite <- Heqn'. apply e2. }
         rewrite H3. rewrite left_el_app. reflexivity.
       * inversion H0.
-    + exists Z0,t. right. left. split. reflexivity. destruct f2. 2:destruct t0.
+    + inversion H0.
+    + inversion H0. subst. destruct H1. reflexivity.
+    + inversion H0.
+  - inversion H.
+  - inversion H.
+(*
+    + exists k,t. right. left. split. reflexivity. destruct f2. 2:destruct t0.
       * inversion H0.
-      * inversion H0. remember (S n) as n'. simpl.
+      * inversion H0.
+      * inversion H0. 
+      * remember (S n) as n'. simpl.
         destruct (point n f) eqn:e1. destruct p.
         destruct (point n' f) eqn:e2. destruct p.
         assert (t4 = tl_app t2 (tl_cons (final t) tl_nil)).
@@ -1404,17 +1169,17 @@ Proof.
     + exists Z0,f1. right. right. split. reflexivity.
       apply point_none in H2. rewrite H2 in H0. inversion H0.
   - inversion H.
-  - inversion H.
+  - inversion H. *)
   - remember (a::cn) as cn1. remember (t::cf) as cf1.
     simpl in H0. rewrite H2 in H0.
-    destruct (next_node cn1 cf1) eqn:e1; try (destruct c);
+    destruct (next_node cn1 cf1) eqn:e1; try (destruct p; destruct c);
     destruct o eqn:e2; destruct f2.
     + destruct l. 2:destruct l0.
       destruct t0. inversion H0. inversion H0. inversion H0. subst. destruct H1. reflexivity.
       destruct t0. inversion H0. inversion H0. inversion H0. subst. destruct H1. reflexivity.
       destruct t0. destruct (point n0 t1) eqn:e3. destruct p.
       destruct o0. destruct t4.
-      { exists k,t0. left. split. reflexivity.
+      { exists k1,t0. left. split. reflexivity.
         inversion H0. remember (n0::l) as cn2. remember (t1::l0) as cf2.
         simpl. rewrite H2. destruct t4. admit. (* shouldn't be possible, cuz a whole nil treelist... *)
         simpl. admit. } (* Actually need to investigate point a t, etc blahhh *)
@@ -1432,9 +1197,413 @@ Proof.
     + admit.
 Admitted.
 
-Theorem cursor_elements_next : forall cn cf c,
+(* Lemma 8 *)
+Theorem next_correct_struct : forall cn cf c k,
+  cursor_correct_struct (cn,cf) -> next_node cn cf = Some (c,k) -> cursor_correct_struct c.
+Proof.
+  induction cn,cf.
+  - intros; simpl. simpl in H0. inversion H0.
+  - intros; simpl. inversion H.
+  - intros; simpl. inversion H.
+  - intros. inversion H.
+    + subst. simpl in H0. destruct (point a t) eqn:e. destruct p.
+      destruct o. destruct t2; destruct t0; try (inversion H0).
+      destruct t0; inversion H0; apply cc_first.
+      apply H.
+      apply cc_first.
+      inversion H0.
+    + subst. remember (n::ci) as cn'. remember (f::ct) as cf'.
+      simpl in H0. destruct (point a t) eqn:e. destruct p.
+      destruct o; destruct t0.
+      * destruct t2. destruct (next_node cn' cf') eqn:e2. destruct p. destruct c0.
+        destruct l. inversion H0. destruct l0. inversion H0.
+        destruct (point n0 t2) eqn:e3. destruct p. destruct o. destruct t5.
+        { inversion H0. apply cc_node with k3. apply IHcn with cf' k2. apply H3. apply e2.
+          apply point_lin_search with t4 t3. apply e3. }
+        { inversion H0. apply cc_final. apply IHcn with cf' k2. apply H3. apply e2.
+          apply point_lin_search with t4 t3. apply e3. }
+        { inversion H0. }
+        { inversion H0. }
+        { inversion H0. }
+        destruct (next_node cn' cf') eqn:e2. destruct p. destruct c0.
+        destruct l. inversion H0. destruct l0. inversion H0.
+        destruct (point n0 t2) eqn:e3. destruct p. destruct o. destruct t5.
+        { inversion H0. apply cc_node with k2. apply IHcn with cf' k1. apply H3. apply e2.
+          apply point_lin_search with t4 t3. apply e3. }
+        { inversion H0. apply cc_final. apply IHcn with cf' k1. apply H3. apply e2.
+          apply point_lin_search with t4 t3. apply e3. }
+        { inversion H0. }
+        { inversion H0. }
+        { inversion H0. }
+        inversion H0. apply H.
+      * destruct t2; destruct t0.
+        { inversion H0. inversion H. apply cc_first. apply cc_node with k3.
+          apply H7. apply H10. apply cc_final. apply H7. apply H10. }
+        { inversion H0. inversion H. apply cc_first. apply cc_node with k2.
+          apply H7. apply H10. apply cc_final. apply H7. apply H10. }
+        destruct (next_node cn' cf') eqn:e2. destruct p. destruct c0.
+        destruct l. inversion H0. destruct l0. inversion H0.
+        destruct (point n0 t0) eqn:e3. destruct p. destruct o. destruct t6.
+        { inversion H0. apply cc_node with k4. apply IHcn with cf' k3. apply H3. apply e2.
+          apply point_lin_search with t5 t4. apply e3. }
+        { inversion H0. apply cc_final. apply IHcn with cf' k3. apply H3. apply e2.
+          apply point_lin_search with t5 t4. apply e3. }
+        { inversion H0. }
+        { inversion H0. }
+        { inversion H0. }
+        destruct (next_node cn' cf') eqn:e2. destruct p. destruct c0.
+        destruct l. inversion H0. destruct l0. inversion H0.
+        destruct (point n0 t4) eqn:e3. destruct p. destruct o. destruct t7.
+        { inversion H0. apply cc_node with k3. apply IHcn with cf' k2. apply H3. apply e2.
+          apply point_lin_search with t6 t5. apply e3. }
+        { inversion H0. apply cc_final. apply IHcn with cf' k2. apply H3. apply e2.
+          apply point_lin_search with t6 t5. apply e3. }
+        { inversion H0. }
+        { inversion H0. }
+        { inversion H0. }
+        destruct (next_node cn' cf') eqn:e2. destruct p. destruct c0.
+        destruct l. inversion H0. destruct l0. inversion H0.
+        destruct (point n0 t4) eqn:e3. destruct p. destruct o. destruct t7.
+        { inversion H0. apply cc_node with k2. apply IHcn with cf' k1. apply H3. apply e2.
+          apply point_lin_search with t6 t5. apply e3. }
+        { inversion H0. apply cc_final. apply IHcn with cf' k1. apply H3. apply e2.
+          apply point_lin_search with t6 t5. apply e3. }
+        { inversion H0. }
+        { inversion H0. }
+        { inversion H0. }
+        destruct (next_node cn' cf') eqn:e2. destruct p. destruct c0.
+        destruct l. inversion H0. destruct l0. inversion H0.
+        destruct (point n0 t0) eqn:e3. destruct p. destruct o. destruct t6.
+        { inversion H0. apply cc_node with k3. apply IHcn with cf' k2. apply H3. apply e2.
+          apply point_lin_search with t5 t4. apply e3. }
+        { inversion H0. apply cc_final. apply IHcn with cf' k2. apply H3. apply e2.
+          apply point_lin_search with t5 t4. apply e3. }
+        { inversion H0. }
+        { inversion H0. }
+        { inversion H0. }
+        { inversion H0. inversion H. apply cc_first. apply cc_node with k3.
+          apply H7. apply H10. apply cc_final. apply H7. apply H10. }
+        { inversion H0. inversion H. apply cc_first. apply cc_node with k2.
+          apply H7. apply H10. apply cc_final. apply H7. apply H10. }
+        { inversion H0. inversion H. apply cc_first. apply cc_node with k3.
+          apply H7. apply H10. apply cc_final. apply H7. apply H10. }
+      * destruct (next_node cn' cf') eqn:e2. destruct p. destruct c0.
+        destruct l. inversion H0. destruct l0. inversion H0.
+        destruct (point n0 t0) eqn:e3. destruct p. destruct o. destruct t4.
+        { inversion H0. apply cc_node with k2. apply IHcn with cf' k1. apply H3. apply e2.
+          apply point_lin_search with t3 t2. apply e3. }
+        { inversion H0. apply cc_final. apply IHcn with cf' k1. apply H3. apply e2.
+          apply point_lin_search with t3 t2. apply e3. }
+        { inversion H0. }
+        { inversion H0. }
+        { inversion H0. }
+      * apply point_none in e. inversion e.
+    + subst. remember (n::ci) as cn'. remember (f::ct) as cf'.
+      simpl in H0. destruct (point a t) eqn:e. destruct p.
+      destruct o; destruct t0.
+      * destruct t2. destruct (next_node cn' cf') eqn:e2. destruct p. destruct c0.
+        destruct l. inversion H0. destruct l0. inversion H0.
+        destruct (point n0 t2) eqn:e3. destruct p. destruct o. destruct t5.
+        { inversion H0. apply cc_node with k2. apply IHcn with cf' k1. apply H3. apply e2.
+          apply point_lin_search with t4 t3. apply e3. }
+        { inversion H0. apply cc_final. apply IHcn with cf' k1. apply H3. apply e2.
+          apply point_lin_search with t4 t3. apply e3. }
+        { inversion H0. }
+        { inversion H0. }
+        { inversion H0. }
+        destruct (next_node cn' cf') eqn:e2. destruct p. destruct c0.
+        destruct l. inversion H0. destruct l0. inversion H0.
+        destruct (point n0 t2) eqn:e3. destruct p. destruct o. destruct t5.
+        { inversion H0. apply cc_node with k1. apply IHcn with cf' k0. apply H3. apply e2.
+          apply point_lin_search with t4 t3. apply e3. }
+        { inversion H0. apply cc_final. apply IHcn with cf' k0. apply H3. apply e2.
+          apply point_lin_search with t4 t3. apply e3. }
+        { inversion H0. }
+        { inversion H0. }
+        { inversion H0. }
+        inversion H0. apply H.
+      * destruct t2; destruct t0.
+        { inversion H0. inversion H. apply cc_first. apply cc_node with k2.
+          apply H7. apply H10. apply cc_final. apply H7. apply H10. }
+        { inversion H0. inversion H. apply cc_first. apply cc_node with k1.
+          apply H7. apply H10. apply cc_final. apply H7. apply H10. }
+        destruct (next_node cn' cf') eqn:e2. destruct p. destruct c0.
+        destruct l. inversion H0. destruct l0. inversion H0.
+        destruct (point n0 t0) eqn:e3. destruct p. destruct o. destruct t6.
+        { inversion H0. apply cc_node with k3. apply IHcn with cf' k2. apply H3. apply e2.
+          apply point_lin_search with t5 t4. apply e3. }
+        { inversion H0. apply cc_final. apply IHcn with cf' k2. apply H3. apply e2.
+          apply point_lin_search with t5 t4. apply e3. }
+        { inversion H0. }
+        { inversion H0. }
+        { inversion H0. }
+        destruct (next_node cn' cf') eqn:e2. destruct p. destruct c0.
+        destruct l. inversion H0. destruct l0. inversion H0.
+        destruct (point n0 t4) eqn:e3. destruct p. destruct o. destruct t7.
+        { inversion H0. apply cc_node with k2. apply IHcn with cf' k1. apply H3. apply e2.
+          apply point_lin_search with t6 t5. apply e3. }
+        { inversion H0. apply cc_final. apply IHcn with cf' k1. apply H3. apply e2.
+          apply point_lin_search with t6 t5. apply e3. }
+        { inversion H0. }
+        { inversion H0. }
+        { inversion H0. }
+        destruct (next_node cn' cf') eqn:e2. destruct p. destruct c0.
+        destruct l. inversion H0. destruct l0. inversion H0.
+        destruct (point n0 t4) eqn:e3. destruct p. destruct o. destruct t7.
+        { inversion H0. apply cc_node with k1. apply IHcn with cf' k0. apply H3. apply e2.
+          apply point_lin_search with t6 t5. apply e3. }
+        { inversion H0. apply cc_final. apply IHcn with cf' k0. apply H3. apply e2.
+          apply point_lin_search with t6 t5. apply e3. }
+        { inversion H0. }
+        { inversion H0. }
+        { inversion H0. }
+        destruct (next_node cn' cf') eqn:e2. destruct p. destruct c0.
+        destruct l. inversion H0. destruct l0. inversion H0.
+        destruct (point n0 t0) eqn:e3. destruct p. destruct o. destruct t6.
+        { inversion H0. apply cc_node with k2. apply IHcn with cf' k1. apply H3. apply e2.
+          apply point_lin_search with t5 t4. apply e3. }
+        { inversion H0. apply cc_final. apply IHcn with cf' k1. apply H3. apply e2.
+          apply point_lin_search with t5 t4. apply e3. }
+        { inversion H0. }
+        { inversion H0. }
+        { inversion H0. }
+        { inversion H0. inversion H. apply cc_first. apply cc_node with k2.
+          apply H7. apply H10. apply cc_final. apply H7. apply H10. }
+        { inversion H0. inversion H. apply cc_first. apply cc_node with k1.
+          apply H7. apply H10. apply cc_final. apply H7. apply H10. }
+        { inversion H0. inversion H. apply cc_first. apply cc_node with k2.
+          apply H7. apply H10. apply cc_final. apply H7. apply H10. }
+      * destruct (next_node cn' cf') eqn:e2. destruct p. destruct c0.
+        destruct l. inversion H0. destruct l0. inversion H0.
+        destruct (point n0 t0) eqn:e3. destruct p. destruct o. destruct t4.
+        { inversion H0. apply cc_node with k1. apply IHcn with cf' k0. apply H3. apply e2.
+          apply point_lin_search with t3 t2. apply e3. }
+        { inversion H0. apply cc_final. apply IHcn with cf' k0. apply H3. apply e2.
+          apply point_lin_search with t3 t2. apply e3. }
+        { inversion H0. }
+        { inversion H0. }
+        { inversion H0. }
+      * apply point_none in e. inversion e.
+Qed.
+
+(* Helper for Lemma 8 *)
+Lemma balance_carries_one : forall n f k f',
+  balanced f ->
+  (lin_search n f = Some (node k f') \/ lin_search n f = Some (final f')) ->
+  balanced f'.
+Proof.
+  induction n; intros; destruct f.
+  - inversion H0; inversion H1.
+  - inversion H0; inversion H1; rewrite H3 in H; inversion H; inversion H2; subst.
+    unfold balanced. exists n. apply H7.
+    unfold balanced. exists n. apply H6.
+  - inversion H0; inversion H1.
+  - simpl in H0. apply IHn with f k.
+    + inversion H. inversion H1; subst.
+      exists 1. apply H4.
+      exists (S n0). apply H6.
+      exists 1. apply bf_nil.
+    + apply H0.
+Qed.
+
+(* Helper for Lemma 8 *)
+Lemma balance_carries : forall cn cf n f,
+  cursor_correct_struct (n::cn,f::cf) ->
+  rec_prop balanced (cn,cf) ->
+  cn <> [] ->
+  rec_prop balanced (n::cn,f::cf).
+Proof.
+  intros. inversion H0. destruct H1. auto.
+  subst. apply rp_next. 2:apply H0.
+  inversion H4. inversion H.
+  - subst. apply balance_carries_one with n0 f0 k. apply H4. left. apply H12.
+  - subst. apply balance_carries_one with n0 f0 Z0. apply H4. right. apply H12.
+Qed.
+
+(* Lemma 8 *)
+Theorem next_node_balanced : forall cn cf c k,
+  cursor_correct_struct (cn,cf) -> rec_prop balanced (cn,cf) ->
+  next_node cn cf = Some (c,k) -> rec_prop balanced c.
+Proof.
+  induction cn,cf; intros.
+  - inversion H1.
+  - inversion H1.
+  - inversion H1.
+  - inversion H0. subst.
+    assert (cursor_correct_struct (cn,cf)).
+    { inversion H; subst. apply cc_nil. apply H5. apply H5. }
+    assert (IHpart: forall c k, next_node cn cf = Some (c,k) -> rec_prop balanced c).
+    { intros. apply IHcn with cf k0. apply H2. apply H7. apply H3. }
+    assert (cursor_correct_struct c).
+    { apply next_correct_struct with (a::cn) (t::cf) k. apply H. apply H1. }
+    inversion H1. destruct (point a t) eqn:e1. destruct p.
+    destruct o; try (destruct t2); destruct t0.
+    + destruct (next_node cn cf) eqn:e2. destruct p. destruct c0. destruct l. 2:destruct l0.
+      inversion H6. inversion H6. destruct (point n t0). destruct p.
+      2:inversion H6. destruct o. 2:inversion H6. destruct t5. 3:inversion H6.
+      * inversion H6. apply balance_carries.
+        rewrite H8. apply H3.
+        apply IHpart with k1. reflexivity.
+        intros Hcontra. inversion Hcontra.
+      * inversion H6. apply balance_carries.
+        rewrite H8. apply H3.
+        apply IHpart with k1. reflexivity.
+        intros Hcontra. inversion Hcontra.
+    + destruct t0.
+      { inversion H6. apply rp_next. apply H4. apply H7. }
+      { inversion H6. apply rp_next. apply H4. apply H7. }
+      destruct (next_node cn cf) eqn:e2. destruct p. destruct c0. destruct l. 2:destruct l0.
+      inversion H6. inversion H6. 2:inversion H6.
+      destruct (point n t0) eqn:e3. destruct p. destruct o. destruct t6.
+      { inversion H6. apply balance_carries.
+        rewrite H8. apply H3.
+        apply IHpart with k2. reflexivity.
+        intros Hcontra. inversion Hcontra. }
+      { inversion H6. apply balance_carries.
+        rewrite H8. apply H3.
+        apply IHpart with k2. reflexivity.
+        intros Hcontra. inversion Hcontra. }
+      inversion H6. inversion H6.
+    + destruct (next_node cn cf) eqn:e2. destruct p. destruct c0. destruct l. 2:destruct l0.
+      inversion H6. inversion H6. destruct (point n t0). destruct p.
+      2:inversion H6. destruct o. 2:inversion H6. destruct t5. 3:inversion H6.
+      * inversion H6. apply balance_carries.
+        rewrite H8. apply H3.
+        apply IHpart with k0. reflexivity.
+        intros Hcontra. inversion Hcontra.
+      * inversion H6. apply balance_carries.
+        rewrite H8. apply H3.
+        apply IHpart with k0. reflexivity.
+        intros Hcontra. inversion Hcontra.
+    + destruct (next_node cn cf) eqn:e2. destruct p. destruct c0. destruct l. 2:destruct l0.
+      inversion H6. inversion H6. destruct (point n t4). destruct p.
+      2:inversion H6. destruct o. 2:inversion H6. destruct t7. 3:inversion H6.
+      * inversion H6. apply balance_carries.
+        rewrite H8. apply H3.
+        apply IHpart with k0. reflexivity.
+        intros Hcontra. inversion Hcontra.
+      * inversion H6. apply balance_carries.
+        rewrite H8. apply H3.
+        apply IHpart with k0. reflexivity.
+        intros Hcontra. inversion Hcontra.
+    + inversion H6. apply H0.
+    + inversion H6. apply H0.
+    + destruct (next_node cn cf) eqn:e2. destruct p. destruct c0. destruct l. 2:destruct l0.
+      inversion H6. inversion H6. destruct (point n t0). destruct p.
+      2:inversion H6. destruct o. 2:inversion H6. destruct t4. 3:inversion H6.
+      * inversion H6. apply balance_carries.
+        rewrite H8. apply H3.
+        apply IHpart with k0. reflexivity.
+        intros Hcontra. inversion Hcontra.
+      * inversion H6. apply balance_carries.
+        rewrite H8. apply H3.
+        apply IHpart with k0. reflexivity.
+        intros Hcontra. inversion Hcontra.
+    + destruct (next_node cn cf) eqn:e2. destruct p. destruct c0. destruct l. 2:destruct l0.
+      inversion H6. inversion H6. destruct (point n t3). destruct p.
+      2:inversion H6. destruct o. 2:inversion H6. destruct t6. 3:inversion H6.
+      * inversion H6. apply balance_carries.
+        rewrite H8. apply H3.
+        apply IHpart with k0. reflexivity.
+        intros Hcontra. inversion Hcontra.
+      * inversion H6. apply balance_carries.
+        rewrite H8. apply H3.
+        apply IHpart with k0. reflexivity.
+        intros Hcontra. inversion Hcontra.
+Qed.
+
+(* Lemma 8 *)
+Lemma next_node_sorted : forall cn cf c k,
+  cursor_correct_struct (cn,cf) -> rec_prop sorted (cn,cf) ->
+  next_node cn cf = Some (c,k) -> rec_prop sorted c.
+Proof. Admitted.
+
+(* Lemma 8 *)
+Lemma next_node_fanout : forall cn cf c k,
+  cursor_correct_struct (cn,cf) -> rec_prop fanout (cn,cf) ->
+  next_node cn cf = Some (c,k) -> rec_prop fanout c.
+Proof. Admitted.
+
+(* Lemma 8 *)
+Theorem next_node_correct : forall cn cf c k,
+  cursor_correct (cn,cf) -> next_node cn cf = Some (c,k) -> cursor_correct c.
+Proof.
+  intros. destruct H. destruct H1. destruct H2.
+  unfold cursor_correct. split. 2:split. 3:split.
+  - apply next_correct_struct with cn cf k. apply H. apply H0.
+  - apply next_node_balanced with cn cf k. apply H. apply H1. apply H0.
+  - apply next_node_sorted with cn cf k. apply H. apply H2. apply H0.
+  - apply next_node_fanout with cn cf k. apply H. apply H3. apply H0.
+Qed.
+
+Lemma next_node_none : forall cn cf cn' cf' k,
+  next_node cn cf = Some (cn',cf',k) ->
+  cn' <> [] /\ cf' <> [].
+Proof.
+  induction cn,cf; intros.
+  - simpl in H. inversion H.
+  - simpl in H. inversion H.
+  - simpl in H. inversion H.
+  - simpl in H. destruct (point a t) eqn:e. destruct p.
+    destruct t0; destruct o. destruct t0.
+    * destruct (next_node cn cf) eqn:e2. destruct p. destruct c; destruct l. 2:destruct l0.
+      inversion H. inversion H.
+      destruct (point n t2) eqn:e3. destruct p.
+      destruct o; try (destruct t5); inversion H; split; intros Hcontra; inversion Hcontra.
+      inversion H.
+    * destruct (next_node cn cf) eqn:e2. destruct p. destruct c; destruct l. 2:destruct l0.
+      inversion H. inversion H.
+      destruct (point n t2) eqn:e3. destruct p.
+      destruct o; try (destruct t5); inversion H; split; intros Hcontra; inversion Hcontra.
+      inversion H.
+    * inversion H. split; intros Hcontra; inversion Hcontra.
+    * destruct (next_node cn cf) eqn:e2. destruct p. destruct c; destruct l. 2:destruct l0.
+      inversion H. inversion H.
+      destruct (point n t0) eqn:e3. destruct p.
+      destruct o; try (destruct t4); inversion H; split; intros Hcontra; inversion Hcontra.
+      inversion H.
+    * destruct t3; destruct t0.
+      inversion H. split; intros Hcontra; inversion Hcontra.
+      inversion H. split; intros Hcontra; inversion Hcontra.
+      destruct (next_node cn cf) eqn:e2. destruct p. destruct c; destruct l. 2:destruct l0.
+      inversion H. inversion H.
+      destruct (point n t0) eqn:e3. destruct p. destruct o. destruct t6.
+      inversion H. split; intros Hcontra; inversion Hcontra.
+      inversion H. split; intros Hcontra; inversion Hcontra.
+      inversion H. inversion H. inversion H.
+      destruct (next_node cn cf) eqn:e2. destruct p. destruct c; destruct l. 2:destruct l0.
+      inversion H. inversion H.
+      destruct (point n t4) eqn:e3. destruct p. destruct o. destruct t7.
+      inversion H. split; intros Hcontra; inversion Hcontra.
+      inversion H. split; intros Hcontra; inversion Hcontra.
+      inversion H. inversion H. inversion H.
+      destruct (next_node cn cf) eqn:e2. destruct p. destruct c; destruct l. 2:destruct l0.
+      inversion H. inversion H.
+      destruct (point n t4) eqn:e3. destruct p. destruct o. destruct t7.
+      inversion H. split; intros Hcontra; inversion Hcontra.
+      inversion H. split; intros Hcontra; inversion Hcontra.
+      inversion H. inversion H. inversion H.
+      destruct (next_node cn cf) eqn:e2. destruct p. destruct c; destruct l. 2:destruct l0.
+      inversion H. inversion H.
+      destruct (point n t0) eqn:e3. destruct p. destruct o. destruct t6.
+      inversion H. split; intros Hcontra; inversion Hcontra.
+      inversion H. split; intros Hcontra; inversion Hcontra.
+      inversion H. inversion H. inversion H.
+      inversion H. split; intros Hcontra; inversion Hcontra.
+      inversion H. split; intros Hcontra; inversion Hcontra.
+      inversion H. split; intros Hcontra; inversion Hcontra.
+    * destruct (next_node cn cf) eqn:e2. destruct p. destruct c; destruct l. 2:destruct l0.
+      inversion H. inversion H.
+      destruct (point n t3) eqn:e3. destruct p. destruct o. destruct t6.
+      inversion H. split; intros Hcontra; inversion Hcontra.
+      inversion H. split; intros Hcontra; inversion Hcontra.
+      inversion H. inversion H. inversion H.
+Qed.
+
+(* Theorem 9 *)
+Theorem cursor_elements_next : forall cn cf c k,
   cursor_correct_struct (cn,cf) ->
-  next_node cn cf = Some c ->
+  next_node cn cf = Some (c,k) ->
   cursor_elements (cn,cf) = cursor_elements c.
 Proof.
   intros. destruct cn,cf.
@@ -1447,8 +1616,8 @@ Proof.
     + admit. (* ditto *)
     + destruct t0. inversion H0. reflexivity.
       destruct t0. admit. admit. (* ditto *) inversion H0. reflexivity.
-    + destruct t0. destruct (next_node cn cf) eqn:e2. destruct c. destruct c0.
-      destruct l1. 2:destruct l2. inversion H0. inversion H0.
+    + destruct t0. destruct (next_node cn cf) eqn:e2. destruct p. destruct c0.
+      destruct l. 2:destruct l0. inversion H0. inversion H0.
       destruct (point n0 t0) eqn:e3. destruct p. destruct o. destruct t4.
       admit. admit. admit. admit. admit. admit.
 Admitted.
@@ -1514,6 +1683,7 @@ Proof.
     apply IHn with f''. apply H.
 Qed.
 
+(* Theorem 10 *)
 Theorem make_cursor_rec_correct : forall x f' n ci ct n' f,
   cursor_correct_struct (n::ci,f::ct) ->
   dec n' f = f' ->
@@ -1556,6 +1726,7 @@ Proof.
       * apply cc_final. apply H3. apply H6.
 Qed.
 
+(* Theorem 10 *)
 Theorem make_cursor_correct : forall x f,
   cursor_correct_struct (make_cursor x f).
 Proof.
@@ -1564,30 +1735,85 @@ Proof.
   - reflexivity.
 Qed.
 
-Definition mc_val_P (x : key) (t : tree) : Prop := forall k f ci ct n n1 f1 ci' ct' t',
-  t = node k f \/ t = final f ->
-  make_cursor_rec x f ci ct n = (n1::ci',f1::ct') ->
-  lin_search n1 f1 = Some t' ->
-  (exists k v, t = val k v).
+(* Theorem 11 *)
+Theorem make_cursor_right : forall cn cf x f k v l,
+  make_cursor x f = (cn,cf) ->
+  cursor_right cn cf [] = (k,v)::l ->
+  lt_key k x <> true.
+Proof. Admitted.
 
-Theorem make_cursor_val : forall x f t ci ct n n1 f1 ci' ct',
-  make_cursor_rec x f ci ct n = (n1::ci',f1::ct') -> lin_search n1 f1 = Some t -> (exists k v, t = val k v).
+(* Theorem 11 *)
+Theorem make_cursor_left : forall cn cf x f k v l,
+  make_cursor x f = (cn,cf) ->
+  cursor_left cn cf [] = (k,v)::l ->
+  lt_key k x = true.
+Proof. Admitted.
+
+(** Proofs about move_to_next and move_to_prev *)
+
+(* Theorem 12 *)
+Theorem move_to_next_correct : forall c,
+  cursor_correct c ->
+  cursor_correct (move_to_next c).
 Proof.
-  intros x. induction f using treelist_tree_rec with (P := mc_val_P x); try unfold mc_val_P; intros.
-  - inversion H; inversion H2; subst. apply IHf with ci ct n n1 f1 ci' ct'. apply H0. (* apply H1.
-  - inversion H; inversion H2; subst. apply IHf with ci ct n n1 f1 ci' ct'. apply H0. apply H1.
-  - exists k. exists v. reflexivity.
-  - admit.
-  - unfold mc_val_P in IHf. destruct t eqn:e.
-    + simpl in H. destruct (lt_key k x).
-      * apply IHf0 with ci ct (S n) n1 f1 ci' ct'. apply H. apply H0.
-      * apply IHf with k t1 (n::ci) (t1::ct) O n1 f1 ci' ct'. *)
-  admit.
-  - admit.
-  - admit.
-  - admit.
-  - admit.
-Admitted.
+  intros. destruct c. simpl. destruct (next_node l l0) eqn:e.
+  destruct p. destruct c. destruct l1.
+  - apply H.
+  - assert (cursor_correct (n::l1,l2)).
+    { apply next_node_correct with l l0 k. apply H. apply e. }
+    destruct H0. destruct H1. destruct H2.
+    split. 2:split. 3:split.
+    + inversion H0. apply cc_first.
+      apply cc_node with k0. apply H6. apply H8.
+      apply cc_final. apply H6. apply H8.
+    + inversion H1. apply rp_next. apply H6. apply H8.
+    + inversion H2. apply rp_next. apply H6. apply H8.
+    + inversion H3. apply rp_next. apply H6. apply H8.
+  - apply H.
+Qed.
+
+(* Theorem 12 *)
+Theorem move_to_prev_correct : forall c,
+  cursor_correct c ->
+  cursor_correct (move_to_prev c).
+Proof. Admitted.
+
+(* Theorem 13 *)
+Theorem move_to_next_el : forall c l r k v,
+  cursor_correct c ->
+  cursor_elements c = (l,(k,v)::r) ->
+  cursor_elements (move_to_next c) = ((k,v)::l,r).
+Proof. Admitted.
+
+(* Theorem 14 *)
+Theorem move_to_prev_el : forall c l r k v,
+  cursor_correct c ->
+  cursor_elements c = ((k,v)::l,r) ->
+  cursor_elements (move_to_next c) = (l,(k,v)::r).
+Proof. Admitted.
+
+(* Theorem 15 *)
+(* Not 100% on this statement *)
+Theorem move_to_next_none : forall cn cf,
+  cursor_correct (cn,cf) ->
+  (cursor_right cn cf [] = [] <-> move_to_next (cn,cf) = (cn,cf)).
+Proof. Admitted.
+
+(* Theorem 15 *)
+(* ditto *)
+Theorem move_to_prev_none : forall cn cf,
+  cursor_correct (cn,cf) ->
+  (cursor_left cn cf [] = [] <-> move_to_prev (cn,cf) = (cn,cf)).
+Proof. Admitted.
+
+(** Proofs about GET *)
+
+(* Theorem 16 *)
+Theorem get_correct : forall cn cf k v l,
+  cursor_correct (cn,cf) ->
+  cursor_right cn cf [] = (k,v)::l ->
+  get_tree (cn,cf) = Some (val k v).
+Proof. Admitted.
 
 (** Tests *)
 
